add budgeted four-state rans mode

specs/.lake/build/ir/Fastvid.c
@@ -36,6 +36,7 @@ static lean_object* l_Fastvid_reprPredictionMode___closed__11____x40_Fastvid___h
 LEAN_EXPORT lean_object* l___private_Fastvid_0__Fastvid_zigzag_match__1_splitter___redArg___closed__0;
 uint8_t lean_nat_dec_eq(lean_object*, lean_object*);
 static lean_object* l_Fastvid_reprPredictionMode___closed__4____x40_Fastvid___hyg_379_;
+LEAN_EXPORT lean_object* l_Fastvid_ransStateIndex(lean_object*, lean_object*);
 lean_object* lean_nat_to_int(lean_object*);
 lean_object* lean_nat_div(lean_object*, lean_object*);
 LEAN_EXPORT lean_object* l_Fastvid_average2(lean_object*, lean_object*);
@@ -80,6 +81,7 @@ static lean_object* l_Fastvid_zigzag___closed__0;
 static lean_object* l_Fastvid_reprPredictionMode___closed__2____x40_Fastvid___hyg_379_;
 LEAN_EXPORT lean_object* l___private_Fastvid_0__Fastvid_zigzag_match__1_splitter(lean_object*, lean_object*, lean_object*, lean_object*);
 static lean_object* l_Fastvid_reprPredictionMode___closed__8____x40_Fastvid___hyg_379_;
+LEAN_EXPORT lean_object* l_Fastvid_ransStateIndex___boxed(lean_object*, lean_object*);
 static lean_object* l_Fastvid_reprPredictionMode___closed__5____x40_Fastvid___hyg_379_;
 LEAN_EXPORT uint8_t l_Fastvid_PredictionMode_ofNat(lean_object*);
 LEAN_EXPORT lean_object* l_Fastvid_quantStep___boxed(lean_object*, lean_object*);
@@ -1026,6 +1028,24 @@ _start:
 {
 lean_object* x_3; 
 x_3 = l_Fastvid_ransSlot(x_1, x_2);
+lean_dec(x_2);
+lean_dec(x_1);
+return x_3;
+}
+}
+LEAN_EXPORT lean_object* l_Fastvid_ransStateIndex(lean_object* x_1, lean_object* x_2) {
+_start:
+{
+lean_object* x_3; 
+x_3 = lean_nat_mod(x_1, x_2);
+return x_3;
+}
+}
+LEAN_EXPORT lean_object* l_Fastvid_ransStateIndex___boxed(lean_object* x_1, lean_object* x_2) {
+_start:
+{
+lean_object* x_3; 
+x_3 = l_Fastvid_ransStateIndex(x_1, x_2);
 lean_dec(x_2);
 lean_dec(x_1);
 return x_3;
